Add non-rec case to the implementation

Launchbury/CoCallFix.thy
@@ -7,7 +7,24 @@ locale CoCallArityAnalysis =
   fixes cccExp :: "exp \<Rightarrow> (Arity \<rightarrow> AEnv \<times> CoCalls)"
 begin
 definition Aexp :: "exp \<Rightarrow> (Arity \<rightarrow> AEnv)" where "Aexp e = (\<Lambda> a. fst (cccExp e \<cdot> a))"
+
+lemma Aexp_eq:
+  "Aexp e\<cdot>a = fst (cccExp e \<cdot> a)"
+  unfolding Aexp_def by (rule beta_cfun) (intro cont2cont)
+
+lemma fup_Aexp_eq:
+  "fup\<cdot>(Aexp e)\<cdot>a = fst (fup\<cdot>(cccExp e)\<cdot>a)"
+  by (cases a)(simp_all add: Aexp_eq)
+  
+
 definition CCexp :: "exp \<Rightarrow> (Arity \<rightarrow> CoCalls)" where "CCexp \<Gamma> = (\<Lambda> a. snd (cccExp \<Gamma>\<cdot>a))"
+lemma CCexp_eq:
+  "CCexp e\<cdot>a = snd (cccExp e \<cdot> a)"
+  unfolding CCexp_def by (rule beta_cfun) (intro cont2cont)
+
+lemma fup_CCexp_eq:
+  "fup\<cdot>(CCexp e)\<cdot>a = snd (fup\<cdot>(cccExp e)\<cdot>a)"
+  by (cases a)(simp_all add: CCexp_eq)
 
 sublocale ArityAnalysis Aexp.
 sublocale CoCallAnalysis CCexp.
@@ -103,7 +120,7 @@ lemma ccBindsExtra_restr_subst':
   assumes "domA \<Gamma> \<subseteq> S"
   shows  "cc_restr S (ccBindsExtra  \<Gamma>[x::h=y]\<cdot>(ae, G)) 
        = cc_restr S (ccBindsExtra  \<Gamma>\<cdot>(ae f|` S , cc_restr S G))"
-  apply (simp add: ccBindsExtra_simp ccBinds_eq Int_absorb2[OF assms(4)] fv_subst_int[OF assms(3,2)])
+  apply (simp add: ccBindsExtra_simp ccBinds_eq ccBind_eq Int_absorb2[OF assms(4)] fv_subst_int[OF assms(3,2)])
   apply (intro arg_cong2[where f = "op \<squnion>"] refl  arg_cong[OF mapCollect_cong])
   apply (subgoal_tac "k \<in> S")
   apply (auto intro:  ccExp'_restr_subst'[OF assms(1)[OF map_of_SomeD]] simp add: fv_subst_int[OF assms(3,2)]   fv_subst_int2[OF assms(3,2)] ccSquare_def)
@@ -114,7 +131,7 @@ lemma ccBindsExtra_restr:
   assumes "domA \<Gamma> \<subseteq> S"
   shows "cc_restr S (ccBindsExtra \<Gamma>\<cdot>(ae, G)) = cc_restr S (ccBindsExtra \<Gamma>\<cdot>(ae f|` S, cc_restr S G))"
   using assms
-  apply (simp add: ccBindsExtra_simp ccBinds_eq Int_absorb2)
+  apply (simp add: ccBindsExtra_simp ccBinds_eq ccBind_eq Int_absorb2)
   apply (intro arg_cong2[where f = "op \<squnion>"] refl arg_cong[OF mapCollect_cong])
   apply (subgoal_tac "k \<in> S")
   apply simp
@@ -155,10 +172,10 @@ lemma CCfix_restr_subst':
 end
 
 lemma Aexp_eqvt[eqvt]:  "\<pi> \<bullet> (CoCallArityAnalysis.Aexp cccExp e) = CoCallArityAnalysis.Aexp (\<pi> \<bullet> cccExp) (\<pi> \<bullet> e)"
-  unfolding CoCallArityAnalysis.Aexp_def by perm_simp (simp_all add: Abs_cfun_eqvt)
+  apply (rule cfun_eqvtI) unfolding CoCallArityAnalysis.Aexp_eq by perm_simp rule
 
 lemma CCexp_eqvt[eqvt]:  "\<pi> \<bullet> (CoCallArityAnalysis.CCexp cccExp e) = CoCallArityAnalysis.CCexp (\<pi> \<bullet> cccExp) (\<pi> \<bullet> e)"
-  unfolding CoCallArityAnalysis.CCexp_def by perm_simp (simp_all add: Abs_cfun_eqvt)
+  apply (rule cfun_eqvtI) unfolding CoCallArityAnalysis.CCexp_eq by perm_simp rule
 
 (*
 lemma ABindsExtra_eqvt[eqvt]: "\<pi> \<bullet> CoCallArityAnalysis.ABindsExtra = ABindsExtra" sorry
@@ -201,12 +218,15 @@ context CoCallArityAnalysis
 begin
 definition cccFix ::  "heap \<Rightarrow> ((AEnv \<times> CoCalls) \<rightarrow> (AEnv \<times> CoCalls))"
   where "cccFix \<Gamma> = (\<Lambda> i. (Afix \<Gamma>\<cdot>(fst i \<squnion> (\<lambda>_.up\<cdot>0) f|` thunks \<Gamma>), CCfix \<Gamma>\<cdot>(Afix \<Gamma>\<cdot>(fst i  \<squnion> (\<lambda>_.up\<cdot>0) f|` (thunks \<Gamma>)), snd i)))"
+
+lemma cccFix_eq:
+  "cccFix \<Gamma>\<cdot>i = (Afix \<Gamma>\<cdot>(fst i \<squnion> (\<lambda>_.up\<cdot>0) f|` thunks \<Gamma>), CCfix \<Gamma>\<cdot>(Afix \<Gamma>\<cdot>(fst i  \<squnion> (\<lambda>_.up\<cdot>0) f|` (thunks \<Gamma>)), snd i))"
+  unfolding cccFix_def
+  by (rule beta_cfun)(intro cont2cont)
 end
 
 lemma cccFix_eqvt[eqvt]: "\<pi> \<bullet> (CoCallArityAnalysis.cccFix cccExp \<Gamma>) = CoCallArityAnalysis.cccFix  (\<pi> \<bullet> cccExp) (\<pi> \<bullet> \<Gamma>)"
-  unfolding CoCallArityAnalysis.cccFix_def 
-  by perm_simp (simp add: Abs_cfun_eqvt)
-
+  apply (rule cfun_eqvtI) unfolding CoCallArityAnalysis.cccFix_eq by perm_simp rule
 
 lemma cccFix_cong[fundef_cong]:
   "\<lbrakk> (\<And> e. e \<in> snd ` set heap2 \<Longrightarrow> cccexp1 e = cccexp2 e); heap1 = heap2 \<rbrakk>
@@ -217,6 +237,126 @@ lemma cccFix_cong[fundef_cong]:
    apply (rule arg_cong[OF Afix_cong], auto simp add: CoCallArityAnalysis.Aexp_def)[1]
    apply (rule arg_cong2[OF ccFix_cong Afix_cong ])
    apply (auto simp add: CoCallArityAnalysis.Aexp_def)
+   done
+
+
+subsubsection {* The non-recursive case *}
+
+definition ABind_nonrec :: "var \<Rightarrow> exp \<Rightarrow> AEnv \<times> CoCalls \<rightarrow> Arity\<^sub>\<bottom>"
+where
+  "ABind_nonrec x e = (\<Lambda> i. (if isLam e \<or> x--x\<notin>(snd i) then fst i x else up\<cdot>0))"
+
+lemma ABind_nonrec_eq:
+  "ABind_nonrec x e \<cdot> i = (if isLam e \<or> x--x\<notin>(snd i) then fst i x else up\<cdot>0)"
+  unfolding ABind_nonrec_def
+  apply (rule beta_cfun)
+  apply (rule cont_if_else_above)
+  apply auto
+  by (metis in_join join_self_below(4))
+
+lemma ABind_nonrec_eqvt[eqvt]: "\<pi> \<bullet> (ABind_nonrec x e) = ABind_nonrec (\<pi> \<bullet> x) (\<pi> \<bullet> e)"
+  apply (rule cfun_eqvtI)
+  unfolding ABind_nonrec_eq
+  by perm_simp rule
+
+
+
+context CoCallArityAnalysis
+begin
+
+  definition Afix_nonrec
+   where "Afix_nonrec x e = (\<Lambda> i. fup\<cdot>(Aexp e)\<cdot>(ABind_nonrec x e \<cdot> i) \<squnion> fst i)"
+
+  lemma Afix_nonrec_eq[simp]:
+    "Afix_nonrec x e \<cdot> i = fup\<cdot>(Aexp e)\<cdot>(ABind_nonrec x e \<cdot> i) \<squnion> fst i"
+    unfolding Afix_nonrec_def
+    by (rule beta_cfun) simp
+
+  definition CCfix_nonrec
+   where "CCfix_nonrec x e = (\<Lambda> i. ccBind x e \<cdot> i  \<squnion> ccProd (fv e) (ccNeighbors {x} (snd i)) \<squnion> snd i)"
+
+  lemma CCfix_nonrec_eq[simp]:
+    "CCfix_nonrec x e \<cdot> i = ccBind x e \<cdot> i  \<squnion> ccProd (fv e) (ccNeighbors {x} (snd i)) \<squnion> snd i"
+    unfolding CCfix_nonrec_def
+    by (rule beta_cfun) (intro cont2cont)
+
+  definition cccFix_nonrec ::  "var \<Rightarrow> exp \<Rightarrow> ((AEnv \<times> CoCalls) \<rightarrow> (AEnv \<times> CoCalls))"
+    where "cccFix_nonrec x e = (\<Lambda> i. (Afix_nonrec x e \<cdot>i , CCfix_nonrec x e \<cdot>i))"
+
+  lemma cccFix_nonrec_eq[simp]:
+    "cccFix_nonrec x e\<cdot>i = (Afix_nonrec x e \<cdot>i , CCfix_nonrec x e \<cdot>i)"
+    unfolding cccFix_nonrec_def
+    by (rule beta_cfun) (intro cont2cont)
+
+end
+
+
+lemma AFix_nonrec_eqvt[eqvt]: "\<pi> \<bullet> (CoCallArityAnalysis.Afix_nonrec cccExp x e) = CoCallArityAnalysis.Afix_nonrec (\<pi> \<bullet> cccExp) (\<pi> \<bullet> x) (\<pi> \<bullet> e)"
+  apply (rule cfun_eqvtI)
+  unfolding CoCallArityAnalysis.Afix_nonrec_eq
+  by perm_simp rule
+
+
+lemma CCFix_nonrec_eqvt[eqvt]: "\<pi> \<bullet> (CoCallArityAnalysis.CCfix_nonrec cccExp x e) = CoCallArityAnalysis.CCfix_nonrec (\<pi> \<bullet> cccExp) (\<pi> \<bullet> x) (\<pi> \<bullet> e)"
+  apply (rule cfun_eqvtI)
+  unfolding CoCallArityAnalysis.CCfix_nonrec_eq
+  by perm_simp rule
+
+lemma cccFix_nonrec_eqvt[eqvt]: "\<pi> \<bullet> (CoCallArityAnalysis.cccFix_nonrec cccExp x e) = CoCallArityAnalysis.cccFix_nonrec (\<pi> \<bullet> cccExp) (\<pi> \<bullet> x) (\<pi> \<bullet> e)"
+  apply (rule cfun_eqvtI)
+  unfolding CoCallArityAnalysis.cccFix_nonrec_eq
+  by perm_simp rule
+
+subsubsection {* Combining the cases *}
+
+context CoCallArityAnalysis
+begin
+  definition cccFix_choose ::  "heap \<Rightarrow> ((AEnv \<times> CoCalls) \<rightarrow> (AEnv \<times> CoCalls))"
+    where "cccFix_choose \<Gamma> = (if nonrec \<Gamma> then split cccFix_nonrec (hd \<Gamma>) else cccFix \<Gamma>)"
+
+  lemma cccFix_choose_simp1[simp]:
+    "\<not> nonrec \<Gamma> \<Longrightarrow> cccFix_choose \<Gamma> = cccFix \<Gamma>"
+  unfolding cccFix_choose_def by simp
+
+  lemma cccFix_choose_simp2[simp]:
+    "atom x \<sharp> e \<Longrightarrow> cccFix_choose [(x,e)] = cccFix_nonrec x e"
+  unfolding cccFix_choose_def nonrec_def by auto
+
+end
+
+lemma cccFix_choose_eqvt[eqvt]: "\<pi> \<bullet> (CoCallArityAnalysis.cccFix_choose cccExp \<Gamma>) = CoCallArityAnalysis.cccFix_choose (\<pi> \<bullet> cccExp) (\<pi> \<bullet> \<Gamma>)"
+  unfolding CoCallArityAnalysis.cccFix_choose_def 
+  apply (cases nonrec \<pi>  rule: eqvt_cases[where x = \<Gamma>])
+  apply (perm_simp, rule)
+  apply simp
+  apply (erule nonrecE)
+  apply (simp )
+
+  apply simp
+  done
+
+lemma cccFix_nonrec_cong[fundef_cong]:
+  "cccexp1 e = cccexp2 e  \<Longrightarrow> CoCallArityAnalysis.cccFix_nonrec cccexp1 x e = CoCallArityAnalysis.cccFix_nonrec cccexp2 x e"
+   apply (rule cfun_eqI)
+   unfolding CoCallArityAnalysis.cccFix_nonrec_eq
+   unfolding CoCallArityAnalysis.Afix_nonrec_eq
+   unfolding CoCallArityAnalysis.CCfix_nonrec_eq
+   unfolding CoCallArityAnalysis.fup_Aexp_eq
+   apply (simp)
+   apply (rule arg_cong[OF ccBind_cong])
+   apply simp
+   unfolding CoCallArityAnalysis.CCexp_def
+   apply simp
+   done
+
+lemma cccFix_choose_cong[fundef_cong]:
+  "\<lbrakk> (\<And> e. e \<in> snd ` set heap2 \<Longrightarrow> cccexp1 e = cccexp2 e); heap1 = heap2 \<rbrakk>
+      \<Longrightarrow> CoCallArityAnalysis.cccFix_choose cccexp1 heap1 = CoCallArityAnalysis.cccFix_choose cccexp2 heap2"
+   unfolding CoCallArityAnalysis.cccFix_choose_def
+   apply (rule cfun_eqI)
+   apply (auto elim!: nonrecE)
+   apply (rule arg_cong[OF cccFix_nonrec_cong], auto)
+   apply (rule arg_cong[OF cccFix_cong], auto)[1]
    done
 
 end
