Launchbury/CoCallAnalysisImpl.thy
@@ -75,8 +75,8 @@ nominal_function
 where
   "cCCexp (GVar b x) =   (\<Lambda> n . (esing x \<cdot> (up \<cdot> n),                                   \<bottom>))"
 | "cCCexp (Lam [x]. e) = (\<Lambda> n . combined_restrict (fv (Lam [x]. e)) (fst (cCCexp e\<cdot>(pred\<cdot>n)), predCC (fv (Lam [x]. e)) (\<Lambda> a. snd(cCCexp e\<cdot>a))\<cdot>n))"
-| "cCCexp (App e x) =    (\<Lambda> n . (fst (cCCexp e\<cdot>(inc\<cdot>n)) \<squnion> (esing x \<cdot> (up\<cdot>0)),        snd (cCCexp e\<cdot>(inc\<cdot>n)) \<squnion> ccProd {x} (insert x (fv e))))"
-| "cCCexp (Let \<Gamma> e) =    (\<Lambda> n . combined_restrict (fv (Let \<Gamma> e)) (CoCallArityAnalysis.cccFix cCCexp \<Gamma> \<cdot> (cCCexp e\<cdot>n)))"
+| "cCCexp (App e x) =    (\<Lambda> n . (fst (cCCexp e\<cdot>(inc\<cdot>n)) \<squnion> (esing x \<cdot> (up\<cdot>0)),          snd (cCCexp e\<cdot>(inc\<cdot>n)) \<squnion> ccProd {x} (insert x (fv e))))"
+| "cCCexp (Let \<Gamma> e) =    (\<Lambda> n . combined_restrict (fv (Let \<Gamma> e)) (CoCallArityAnalysis.cccFix_choose cCCexp \<Gamma> \<cdot> (cCCexp e\<cdot>n)))"
 proof-
 case goal1
     show ?case
@@ -116,20 +116,21 @@ case (goal13 \<Gamma> body \<Gamma>' body')
     assume *: "supp (-\<pi>) \<sharp>* (fv (Terms.Let \<Gamma> body) :: var set)"
     
     { fix n
-      have "combined_restrict (fv (Terms.Let \<Gamma> body)) (CoCallArityAnalysis.cccFix cCCexp_sumC (\<pi> \<bullet> \<Gamma>)\<cdot>(cCCexp_sumC (\<pi> \<bullet> body)\<cdot>n))
-      =  combined_restrict (fv (Terms.Let \<Gamma> body)) (- \<pi> \<bullet> (CoCallArityAnalysis.cccFix cCCexp_sumC (\<pi> \<bullet> \<Gamma>)\<cdot>(cCCexp_sumC (\<pi> \<bullet> body)\<cdot>n)))"
+      have "combined_restrict (fv (Terms.Let \<Gamma> body)) (CoCallArityAnalysis.cccFix_choose cCCexp_sumC (\<pi> \<bullet> \<Gamma>)\<cdot>(cCCexp_sumC (\<pi> \<bullet> body)\<cdot>n))
+      =  combined_restrict (fv (Terms.Let \<Gamma> body)) (- \<pi> \<bullet> (CoCallArityAnalysis.cccFix_choose cCCexp_sumC (\<pi> \<bullet> \<Gamma>)\<cdot>(cCCexp_sumC (\<pi> \<bullet> body)\<cdot>n)))"
         by (rule combined_restrict_perm[OF *, symmetric]) simp
-      also have "- \<pi> \<bullet> (CoCallArityAnalysis.cccFix cCCexp_sumC (\<pi> \<bullet> \<Gamma>)\<cdot>(cCCexp_sumC (\<pi> \<bullet> body)\<cdot>n)) = 
-                       CoCallArityAnalysis.cccFix (- \<pi> \<bullet> cCCexp_sumC) \<Gamma>\<cdot>((- \<pi> \<bullet> cCCexp_sumC) body\<cdot>n)"
+      also have "- \<pi> \<bullet> (CoCallArityAnalysis.cccFix_choose cCCexp_sumC (\<pi> \<bullet> \<Gamma>)\<cdot>(cCCexp_sumC (\<pi> \<bullet> body)\<cdot>n)) = 
+                       CoCallArityAnalysis.cccFix_choose (- \<pi> \<bullet> cCCexp_sumC) \<Gamma>\<cdot>((- \<pi> \<bullet> cCCexp_sumC) body\<cdot>n)"
         by (simp add: pemute_minus_self)
-      also have "CoCallArityAnalysis.cccFix (- \<pi> \<bullet> cCCexp_sumC) \<Gamma> = CoCallArityAnalysis.cccFix cCCexp_sumC \<Gamma>"
-        by (rule cccFix_cong[OF eqvt_at_apply[OF goal13(1)] refl])
+      also have "CoCallArityAnalysis.cccFix_choose (- \<pi> \<bullet> cCCexp_sumC) \<Gamma> = CoCallArityAnalysis.cccFix_choose cCCexp_sumC \<Gamma>"
+        thm cccFix_cong
+        by (rule cccFix_choose_cong[OF eqvt_at_apply[OF goal13(1)] refl])
       also have "(- \<pi> \<bullet> cCCexp_sumC) body = cCCexp_sumC body"
         by (rule eqvt_at_apply[OF goal13(2)])
       also note calculation
     }
-    thus "(\<Lambda> n. combined_restrict (fv (Terms.Let \<Gamma> body)) (CoCallArityAnalysis.cccFix cCCexp_sumC (\<pi> \<bullet> \<Gamma>)\<cdot>(cCCexp_sumC (\<pi> \<bullet> body)\<cdot>n))) =
-         (\<Lambda> n. combined_restrict (fv (Terms.Let \<Gamma> body)) (CoCallArityAnalysis.cccFix cCCexp_sumC \<Gamma>\<cdot>(cCCexp_sumC body\<cdot>n)))" by (simp only:)
+    thus "(\<Lambda> n. combined_restrict (fv (Terms.Let \<Gamma> body)) (CoCallArityAnalysis.cccFix_choose cCCexp_sumC (\<pi> \<bullet> \<Gamma>)\<cdot>(cCCexp_sumC (\<pi> \<bullet> body)\<cdot>n))) =
+         (\<Lambda> n. combined_restrict (fv (Terms.Let \<Gamma> body)) (CoCallArityAnalysis.cccFix_choose cCCexp_sumC \<Gamma>\<cdot>(cCCexp_sumC body\<cdot>n)))" by (simp only:)
   qed
 qed auto
 
@@ -138,24 +139,37 @@ nominal_termination (eqvt) by lexicographic_order
 
 interpretation CoCallArityAnalysis cCCexp.
 
+lemma cCCexp_eq[simp]:
+  "cCCexp (GVar b x)\<cdot>n =   (esing x \<cdot> (up \<cdot> n),                                   \<bottom>)"
+  "cCCexp (Lam [x]. e)\<cdot>n = combined_restrict (fv (Lam [x]. e)) (fst (cCCexp e\<cdot>(pred\<cdot>n)), predCC (fv (Lam [x]. e)) (\<Lambda> a. snd(cCCexp e\<cdot>a))\<cdot>n)"
+  "cCCexp (App e x)\<cdot>n =    (fst (cCCexp e\<cdot>(inc\<cdot>n)) \<squnion> (esing x \<cdot> (up\<cdot>0)),          snd (cCCexp e\<cdot>(inc\<cdot>n)) \<squnion> ccProd {x} (insert x (fv e)))"
+  "cCCexp (Let \<Gamma> e)\<cdot>n =    combined_restrict (fv (Let \<Gamma> e)) (CoCallArityAnalysis.cccFix_choose cCCexp \<Gamma> \<cdot> (cCCexp e\<cdot>n))"
+by (simp_all)
+declare cCCexp.simps[simp del]
+
+
 lemma Aexp_simps[simp]:
   "Aexp (GVar b x)\<cdot>n = esing x\<cdot>(up\<cdot>n)"
   "Aexp (Lam [x]. e)\<cdot>n = Aexp e\<cdot>(pred\<cdot>n) f|` fv (Lam [x]. e)"
   "Aexp (App e x)\<cdot>n = Aexp e\<cdot>(inc\<cdot>n) \<squnion> esing x\<cdot>(up\<cdot>0)"
-  "Aexp (Let \<Gamma> e)\<cdot>n = (Afix \<Gamma>\<cdot>(Aexp e\<cdot>n \<squnion> (\<lambda>_.up\<cdot>0) f|` thunks \<Gamma>)) f|` (fv (Let \<Gamma> e))"
-unfolding Aexp_def CCexp_def  by (simp add: beta_cfun cccFix_def)+
+  "\<not> nonrec \<Gamma> \<Longrightarrow> Aexp (Let \<Gamma> e)\<cdot>n = (Afix \<Gamma>\<cdot>(Aexp e\<cdot>n \<squnion> (\<lambda>_.up\<cdot>0) f|` thunks \<Gamma>)) f|` (fv (Let \<Gamma> e))"
+  "atom x \<sharp> e \<Longrightarrow> Aexp (let x be e in exp)\<cdot>n = (fup\<cdot>(Aexp e)\<cdot>(ABind_nonrec x e \<cdot> (Aexp exp\<cdot>n, CCexp exp\<cdot>n)) \<squnion> Aexp exp\<cdot>n) f|` (fv (let x be e in exp))"
+ by (simp add: cccFix_eq Aexp_eq fup_Aexp_eq CCexp_eq fup_CCexp_eq)+
+
 
 lemma CCexp_simps[simp]:
   "CCexp (GVar b x)\<cdot>n = \<bottom>"
   "CCexp (Lam [x]. e)\<cdot>n = predCC (fv (Lam [x]. e)) (CCexp e)\<cdot>n"
   "CCexp (App e x)\<cdot>n = CCexp e\<cdot>(inc\<cdot>n) \<squnion> ccProd {x} (insert x (fv e))"
-  "CCexp (Let \<Gamma> e)\<cdot>n = cc_restr (fv (Let \<Gamma> e)) (CCfix \<Gamma>\<cdot>(Afix \<Gamma>\<cdot>(Aexp e\<cdot>n  \<squnion> (\<lambda>_.up\<cdot>0) f|` (thunks \<Gamma>)), CCexp e\<cdot>n))"
-unfolding Aexp_def CCexp_def  by (simp add: beta_cfun cccFix_def)+
+  "\<not> nonrec \<Gamma> \<Longrightarrow> CCexp (Let \<Gamma> e)\<cdot>n = cc_restr (fv (Let \<Gamma> e)) (CCfix \<Gamma>\<cdot>(Afix \<Gamma>\<cdot>(Aexp e\<cdot>n  \<squnion> (\<lambda>_.up\<cdot>0) f|` (thunks \<Gamma>)), CCexp e\<cdot>n))"
+  "atom x \<sharp> e \<Longrightarrow> CCexp (let x be e in exp)\<cdot>n = cc_restr (fv (let x be e in exp)) (ccBind x e \<cdot>(Aexp exp\<cdot>n, CCexp exp\<cdot>n) \<squnion> ccProd (fv e) (ccNeighbors {x} (CCexp exp\<cdot>n)) \<squnion> CCexp exp\<cdot>n)"
+ by (simp add: cccFix_eq Aexp_eq fup_Aexp_eq CCexp_eq fup_CCexp_eq predCC_eq)+
 
 lemma ccField_CCexp:
   "ccField (CCexp e\<cdot>n) \<subseteq> fv e"
-by (induction e arbitrary: n rule: exp_induct)
+by (induction e arbitrary: n rule: exp_induct_rec)
    (auto simp add: ccField_ccProd predCC_eq dest: set_mp[OF ccField_cc_restr])
+
 
 lemma cc_restr_CCexp[simp]:
   "cc_restr (fv e) (CCexp e\<cdot>a) = CCexp e\<cdot>a"
